Environment.v
@@ -6,10 +6,14 @@ Definition loc_ctxt := env unit.
 Definition ty_ctxt := env ty.
 
 (* DbLib utils *)
-Lemma lookup_zero_cons : forall {A} (E : env A) e,
+Lemma lookup_zero_nil : forall A,
+  lookup 0 [] = @None A.
+Proof. auto. Qed.
+
+Lemma lookup_zero_cons : forall A (E : env A) e,
   lookup 0 (e :: E) = e.
 Proof. eauto. Qed.
 
-Lemma lookup_succ_cons : forall {A} (E : env A) e x,
+Lemma lookup_succ_cons : forall A (E : env A) e x,
   lookup (S x) (e :: E) = lookup x E.
 Proof. eauto. Qed.
