Preservation.v
@@ -1,0 +1,46 @@
+Require Import DbLib.Environments.
+Require Import List.
+Require Import Typing.
+Require Import Syntax.
+Require Import Empty.
+Require Import Context.
+Require Import Environment.
+Require Import DbLib.DeBruijn.
+Require Import Arith.
+Require Import DbLibExt.
+Require Import InsertNone.
+Require Import Subst.
+Require Import SmallStepSemantics.
+Import ListNotations.
+
+Theorem preservation : forall L E e e' s s' t,
+  is_empty L ->
+  is_empty E ->
+  L; E |- e ~: t ->
+  step s e s' e' ->
+  L; E |- e' ~: t.
+Proof with eboom.
+  intros L E e e' s s' t EmptyL EmptyE WT ST.
+  generalize dependent L.
+  generalize dependent E.
+  generalize dependent t.
+  induction ST.
+  Case "Beta reduction".
+    intros.
+    inversion WT; subst.
+    assert (is_empty E1 /\ is_empty E2) as [EmptyE1 EmptyE2]...
+    inversion AppPreWT1; subst.
+    (* Establish that the contexts are all the same length and apply substitution lemma *)
+    set (len := length E).
+    assert (length E1 = len)...
+    assert (length E2 = len)...
+    apply substitution with (E1 := E2) (t1 := t1) (E2 := E1)...
+  Case "App1 stepping".
+    intros.
+    inversion WT; subst.
+    assert (is_empty E1 /\ is_empty E2) as [EmptyE1 _]...
+  Case "App2 stepping".
+    intros.
+    inversion WT; subst.
+    assert (is_empty E1 /\ is_empty E2) as [_ EmptyE2]...
+Qed.
