Subst.v
@@ -1,0 +1,233 @@
+Require Import DbLib.Environments.
+Require Import List.
+Require Import Typing.
+Require Import Syntax.
+Require Import Empty.
+Require Import Context.
+Require Import Environment.
+Require Import DbLib.DeBruijn.
+Require Import Arith.
+Require Import DbLibExt.
+Require Import InsertNone.
+Import ListNotations.
+
+Lemma unshift_Abs : forall x t e, unshift x (TAbs t e) = TAbs t (unshift (S x) e).
+Proof with eauto.
+  intros.
+  simpl_lower_goal...
+Qed.
+
+Lemma unshift_App : forall x e1 e2,
+  unshift x (TApp e1 e2) = TApp (unshift x e1) (unshift x e2).
+Proof with auto.
+  intros.
+  simpl_lower_goal...
+Qed.
+
+Lemma subst_unshift : forall x e v,
+  ~ contains_var x e ->
+  subst v x e = unshift x e.
+Proof with (eauto using f_equal, not_contains_Abs,
+                        not_contains_App1, not_contains_App2 with l3).
+  Local Transparent lower.
+  intros x e v NotContains.
+  generalize dependent x.
+  generalize dependent v.
+  induction e; try solve [simpl_subst_goal; simpl; auto].
+  Case "Var".
+    intros.
+    simpl_subst_goal. simpl.
+    destruct (le_gt_dec x n).
+    SCase "x <= n".
+      destruct (le_lt_eq_dec x n)...
+      SSCase "x < n". subst_idx...
+      SSCase "x = n". exfalso. subst...
+    SCase "x > n".
+      subst_idx...
+  Case "Abs".
+    intros.
+    simpl_subst_goal. rewrite unshift_Abs...
+  Case "App".
+    intros.
+    simpl_subst_goal. rewrite unshift_App.
+    rewrite IHe1...
+Qed.
+
+Lemma typing_without_var : forall L E e x t,
+  L; raw_insert x None E |- e ~: t -> ~ contains_var x e.
+Proof with (eauto using raw_insert_eq_insert_1, le_0_n).
+  unfold not.
+  intros L E e x t WT Contains.
+  generalize dependent E.
+  generalize dependent x.
+  generalize dependent t.
+  induction e; try solve [intros; solve by inversion].
+  Case "Var".
+    intros.
+    destruct (eq_nat_dec x n).
+    SCase "x = n".
+      subst x.
+      inversion WT; subst.
+      assert (Some t = None)...
+      solve by inversion.
+    SCase "x <> n".
+      inversion Contains...
+  Case "TAbs".
+    intros.
+    inversion WT; subst.
+    rewrite insert_insert in AbsPre...
+    inversion Contains; subst...
+  Case "TApp".
+    intros.
+    inversion Contains.
+    (* TODO: deduplicate *)
+    SCase "e1 contains x".
+      subst.
+      inversion WT. subst.
+      apply insert_none_split_backwards in AppPreSplit.
+      decompose record AppPreSplit.
+      subst...
+    SCase "e2 contains x".
+      subst.
+      inversion WT. subst.
+      apply insert_none_split_backwards in AppPreSplit.
+      decompose record AppPreSplit.
+      subst...
+Qed.
+
+Lemma typing_insert_none_subst : forall L E e x junk t,
+  L; raw_insert x None E |- e ~: t ->
+  L; E |- subst junk x e ~: t.
+Proof.
+  intros L E e x junk t WT.
+  remember WT as H eqn:Junk; clear Junk.
+  apply typing_without_var in H.
+  apply subst_unshift with (v := junk) in H.
+  rewrite H.
+  eauto using typing_insert_none_reverse.
+Qed.
+
+Lemma length_zero_nil : forall A (l : list A),
+  length l = length (@nil A) ->
+  l = (@nil A).
+Proof.
+  intros. destruct l; try solve by inversion; reflexivity.
+Qed.
+
+Hint Immediate length_zero_nil : l3.
+
+Lemma context_split_insert : forall A (E : env A) E1 E2 x t,
+  context_split (insert x t E) E1 E2 ->
+  (exists E1' E2',
+    E1 = insert x t E1' /\
+    E2 = raw_insert x None E2' /\
+    length E1' = length E /\
+    length E2' = length E /\
+    context_split E E1' E2'
+  ) \/
+  (exists E1' E2',
+    E1 = raw_insert x None E1' /\
+    E2 = insert x t E2' /\
+    length E1' = length E /\
+    length E2' = length E /\
+    context_split E E1' E2'
+  ).
+Proof with eboom.
+  intros A E E1 E2 x t Split.
+  generalize dependent E.
+  generalize dependent E1.
+  generalize dependent E2.
+  induction x as [|x'].
+  Case "x = 0".
+    intros.
+    rewrite raw_insert_zero in Split.
+    inversion Split; subst.
+    inversion SplitElem; subst; [left | right];
+    eexists; eexists; repeat rewrite raw_insert_zero; repeat split...
+  Case "x = S x'".
+    intros.
+    rewrite raw_insert_successor in Split.
+    destruct E as [|e E];
+    destruct E1 as [|e1 E1'];
+    destruct E2 as [|e2 E2']; try solve by inversion.
+    SCase "E = nil, E1 = e1 :: E1, E2 = e2 :: E2".
+      replace (lookup 0 (@nil (option ty))) with (@None ty) in Split...
+      simpl in *.
+      inversion Split; subst.
+      set (Intro := SplitPre).
+      apply IHx' in Intro...
+      destruct Intro as [IH | IH];
+        [left | right];
+        destruct IH as [E1'' [E2'' [? [? [? [? ?]]]]]];
+        assert (E1'' = []); eboom;
+        assert (E2'' = []); eboom;
+        subst;
+        exists [], [];
+        repeat rewrite raw_insert_successor;
+        repeat rewrite lookup_zero_nil in *;
+        inversion SplitElem...
+  SCase "all cons".
+    rewrite lookup_zero_cons in Split.
+    simpl in Split.
+    inversion Split; subst.
+    set (Intro := SplitPre).
+    apply IHx' in Intro.
+    destruct Intro as [IH | IH];
+      [left | right];
+      destruct IH as [E1'' [E2'' [? [? [? [? ?]]]]]];
+      exists (e1 :: E1''), (e2 :: E2'');
+      repeat rewrite raw_insert_successor in *;
+      repeat rewrite lookup_zero_cons in *;
+      simpl; subst; repeat split...
+Qed.
+
+Lemma substitution: forall L E2 e2 t1 t2 x,
+  L; insert x t1 E2 |- e2 ~: t2 ->
+  forall E E1 e1, L; E1 |- e1 ~: t1 ->
+  context_split E E1 E2 ->
+  L; E |- (subst e1 x e2) ~: t2.
+Proof with (eauto using typing_insert_none, typing_insert_none_subst,
+            split_rotate  with l3).
+  intros L E2 e2 t1 t2 x WT2 E E1 e1 WT1 Split.
+  dependent induction WT2; simpl_subst_goal; try solve [exfalso; eauto using empty_insert_contra].
+  Case "Var".
+    (* XXX: naming of x is weird here *)
+    apply empty_insert_injective in x...
+    destruct x as [XEq [TEq E2Eq]].
+    subst.
+    simpl_subst_goal.
+    apply split_all_left in Split...
+    subst...
+  Case "Abs".
+    constructor.
+    (* XXX: Bug (?) in error reporting - can't specify E0 *)
+    eapply IHWT2 with (t3 := t1) (E1 := (None :: E1)).
+    SCase "inserts are equal". insert_insert.
+    SCase "e1 well-typed under shifting".
+      assert (L; raw_insert 0 None E1 |- shift 0 e1 ~: t1)...
+    SCase "context_split is sensible".
+      rewrite raw_insert_zero; rewrite raw_insert_zero...
+  Case "App".
+    rename E0 into E2'.
+    rename E1 into E1'.
+    rename E3 into E0.
+    rename E2 into E12.
+    (* x is either in E1' or E2' *)
+    assert (SplitX := AppPreSplit).
+    apply context_split_insert in SplitX.
+    destruct SplitX as [XLeft | XRight].
+    SCase "x on the left".
+      destruct XLeft as [E1 [E2 [? [? [? [? ?]]]]]].
+      subst E1'.
+      subst E2'.
+      assert (context_split E12 E2 E1); [eboom | ].
+      assert (exists E01, context_split E E2 E01 /\ context_split E01 E0 E1)
+        as [E01 [Split201 SplitE01]]...
+    SCase "x on the right".
+      destruct XRight as [E1 [E2 [? [? [? [? ?]]]]]].
+      subst E1'.
+      subst E2'.
+      assert (context_split E12 E1 E2); [eboom | ].
+      assert (exists E02, context_split E E1 E02 /\ context_split E02 E0 E2)
+        as [E01 [Split201 SplitE01]]...
+Qed.
